code/experimental/P256/Hacl.Spec.P256.Normalisation.fst
@@ -24,21 +24,26 @@ open Lib.Loops
 open FStar.Math.Lemmas
 
 module B = LowStar.Buffer
+ 
 
+let modp_inv2_pow (x: nat) : Tot (r: nat {r < prime}) = 
+   power_distributivity x (prime - 2) prime;
+   pow x (prime - 2) % prime
 
-let _norm p =
+let _norm (p : nat * nat * nat) =
   let open FStar.Mul in 
   let (x, y, z) = p in
-  let z2 = z * z % prime in 
-  let z2i = modp_inv2 z in 
-  let z3 = z * z *  z % prime in 
-  let z3i = modp_inv2 z3 in 
-  let x3 = (x * z2i) % prime in 
-  let y3 = (y * z3i) % prime in 
+  let z2 = z * z in 
+  let z2i = modp_inv2_pow z2 in 
+  let z3 = z * z * z in 
+  let z3i = modp_inv2_pow z3 in 
+  let x3 = (z2i * x) % prime in 
+  let y3 = (z3i * y) % prime in 
   let z3 = 1 in 
+  assert(x3 == (x * (pow (z * z) (prime -2) % prime) % prime));
   (x3, y3, z3)
 
 open FStar.Mul
 
 (* z * z * pow2 256 * z % prime *)
-val lemma_1: z: nat-> Lemma (toDomain_ (fromDomain_ ((z * z % prime) * pow2 256 % prime) * z % prime) == toDomain_ (z * z * z % prime)) 
+val lemma_1: z: nat-> Lemma (toDomain_ (fromDomain_ (toDomain_ (z * z % prime)) * z % prime) == toDomain_ (z * z * z % prime))
