code/experimental/P256/Hacl.Spec.P256.MontgomeryMultiplication.fsti
@@ -52,6 +52,9 @@ noextract
 val pow: a:nat -> b:nat -> res:nat
 
 
+val power_distributivity: a: nat -> b: nat -> c: pos -> Lemma ((pow (a % c) b) % c = (pow a b) % c)
+
+
 noextract 
 val felem_add_seq: a: felem_seq{felem_seq_as_nat a < prime} -> b: felem_seq{felem_seq_as_nat b < prime} -> 
   Tot (r: felem_seq {felem_seq_as_nat r < prime /\ felem_seq_as_nat r = toDomain_ ((fromDomain_ (felem_seq_as_nat a) + fromDomain_ (felem_seq_as_nat b)) % prime)})
